src/OeufProof.v
@@ -3,8 +3,11 @@ Require Import CompilationUnit.
 Require Import HList.
 Require Import Untyped.
 Require Import StepLib.
-Require Import Semantics.
-        
+Require Import MixSemantics.
+
+Require Import SourceLang.
+
+
 Require Import compcert.lib.Coqlib.
 Require Import compcert.ia32.Asm.
 Require Import compcert.common.AST.
@@ -18,84 +21,35 @@ Require Import StructTact.Util.
 
 Require Import EricTact.
 
-
-(*
- We need some kind of semantics notion for Oeuf programs
-Let's try using a modified version of CompCert's, and see what happens
- 
-*)
-
-
-
-(*
-We're going to need a few things:
-1. a simulation from SourceLang to Flattened, which all use no traces
-2. a simulation from Fmajor to Asm, which all use traces
-3. some way to hook it all up together
-*)
-
-(*
 Section Simulation.
 
   Variable prog : compilation_unit.
   Variable tprog : Asm.program.
   Hypothesis TRANSF : transf_to_asm prog = OK tprog.
 
+  Theorem Oeuf_forward_simulation :
+    forall ty,
+      mix_forward_simulation (@CompilationUnit.source_semantics ty prog) (Asm.semantics tprog).
+  Proof.
+  Admitted.
 
+  Theorem Oeuf_step_sim :
+    forall ty expr expr',
+      Semantics.star _ _ (fun _ => SourceLang.step) tt expr expr' ->
+      forall st i,
+        CompilationUnit.initial_state prog nil ty expr ->
+        Asm.initial_state tprog st ->
+        Oeuf_forward_simulation ty i expr st ->
+        exists st' i',
+          star Asm.step (Genv.globalenv tprog) st E0 st' /\
+          Oeuf_forward_simulation ty i' expr' st'.
+    Proof.
+      intros.
+      edestruct MixSemantics.simulation_star; eauto.
+      simpl. eassumption.
+      break_exists. break_and.
+      repeat eexists; eauto.
+    Qed.
 
-  Lemma fsim :
-    forward_simulation (SourceLang.semantics prog) (Asm.semantics tprog).
   
-Lemma star_step_sim :
-  forall {tys ty} (exp exp' : SourceLang.expr tys ty),
-    sstar SourceLang.step exp exp' ->
-    forall st,
-      match_states exp st ->
-      exists st',
-        star Asm.step ge st E0 st' /\
-        match_states exp' st'.
-Proof.
-  induction 1; intros.
-  solve [eexists; split; eauto; eapply star_refl].
-  eapply step_sim in H; eauto.
-  break_exists. break_and.
-  app plus_star plus.
-  destruct (IHsstar x); eauto.
-  break_and. eexists; split;
-               try eapply H5.
-  eapply star_trans; eauto.
-Qed.
-  
-
-Theorem Oeuf_sim :
-  forall tys ty expr expr',
-    sstar SourceLang.step expr expr' ->
-    forall st,
-      CompilationUnit.initial_state prog tys ty expr ->
-      Asm.initial_state tprog st ->
-      correspond expr st ->
-      exists st',
-        star Asm.step ge st E0 st' /\
-        correspond expr' st'.
-Proof.
-  intros.
-  eapply correspond_initial_match in H2; eauto.
-  eapply star_step_sim in H; eauto.
-  break_exists. break_and.
-  eexists; split; eauto.
-  eapply match_correspond; eauto.
-Qed.
-
-Theorem Oeuf_correspond_exists :
-  forall cu asmprog,
-    transf_to_asm cu = OK asmprog ->
-    forall tys ty expr,
-      CompilationUnit.initial_state cu tys ty expr ->
-      exists st,
-        Asm.initial_state asmprog st /\ 
-        correspond expr st.
-Proof.
-Admitted.
-
 End Simulation.
-*)
